BrownianMotion/Choquet/AnalyticSet.lean
@@ -72,7 +72,7 @@ lemma IsPavingAnalyticFor.exists_memSigma_superset (hs : IsPavingAnalyticFor p �
     ∃ t, t ∈ memSigma p ∧ s ⊆ t := by
   obtain ⟨q, hq_empty, hq_compact, B, hB_prod, rfl⟩ := hs
   rw [memProdSigmaDelta_iff] at hB_prod
-  obtain ⟨A, K, hA, hK, rfl⟩ := hB_prod
+  obtain ⟨A, hA, K, hK, rfl⟩ := hB_prod
   refine ⟨⋃ m, A 0 m, ?_, ?_⟩
   · exact ⟨fun m ↦ A 0 m, fun m ↦ hA 0 m, rfl⟩
   · intro x hx
@@ -125,8 +125,8 @@ lemma IsPavingAnalyticFor.iInter {𝓚 : ℕ → Type*} {s : ℕ → Set 𝓧}
   · refine memDelta.iInter fun n ↦ ?_
     rw [← memProdSigmaDelta]
     simp_rw [memProdSigmaDelta_iff] at hB_prod ⊢
-    choose A K hA hK hB_eq using hB_prod
-    refine ⟨A n, fun i j ↦ {y | y n ∈ K n i j}, hA n, fun i j ↦ ?_, ?_⟩
+    choose A hA K hK hB_eq using hB_prod
+    refine ⟨A n, hA n, fun i j ↦ {y | y n ∈ K n i j}, fun i j ↦ ?_, ?_⟩
     · simp only [Set.mem_image, Set.mem_pi, Set.mem_univ, Set.mem_setOf_eq, forall_const, q']
       rcases Set.eq_empty_or_nonempty (K n i j) with hK_empty | hK_nonempty
       · simp only [hK_empty, Set.mem_empty_iff_false, Set.setOf_false]
@@ -182,7 +182,7 @@ lemma IsPavingAnalyticFor.iUnion {𝓚 : ℕ → Type*} {s : ℕ → Set 𝓧}
     rw [hC_eq]
     refine memDelta.iInter fun k ↦ memDelta_of_mem ?_
     simp_rw [memSigma_memProd_iff] at hA
-    choose B K hB hK hA_eq using hA
+    choose B hB K hK hA_eq using hA
     simp_rw [hA_eq]
     have h_eq : Prod.swap '' ((Equiv.sigmaProdDistrib 𝓚 𝓧).symm '' Set.univ.sigma
         fun n ↦ Prod.swap '' ⋃ n_1, B n k n_1 ×ˢ K n k n_1)
@@ -193,7 +193,7 @@ lemma IsPavingAnalyticFor.iUnion {𝓚 : ℕ → Type*} {s : ℕ → Set 𝓧}
     simp only [Set.image_swap_prod, Set.sigma_eq_biUnion, Set.mem_univ, Set.iUnion_true,
       Set.image_iUnion]
     refine memSigma.iUnion fun j ↦ memSigma_of_mem ?_
-    refine ⟨B j k i, Sigma.mk j '' (K j k i), hB _ _ _, ?_, ?_⟩
+    refine ⟨B j k i, hB _ _ _, Sigma.mk j '' (K j k i), ?_, ?_⟩
     · simp only [Set.mem_image, Set.mem_pi, Set.mem_univ, Set.mem_setOf_eq, forall_const, q'']
       refine ⟨{j}, fun j ↦ K j k i, ?_⟩
       simp only [Finset.coe_singleton, Set.singleton_sigma, and_true]
@@ -229,9 +229,9 @@ lemma IsPavingAnalyticFor.inter {𝓚' : Type*} {t : Set 𝓧}
   · refine memDelta.inter ?_ ?_
     · rw [← memProdSigmaDelta]
       simp_rw [memProdSigmaDelta_iff] at hB_prod ⊢
-      choose A K hA hK hB_eq using hB_prod
-      refine ⟨A, fun i j ↦ {y | y.1 ∈ K i j}, hA, fun i j ↦ ?_, ?_⟩
-      · simp only [memProd, exists_and_left, q'']
+      choose A hA K hK hB_eq using hB_prod
+      refine ⟨A, hA, fun i j ↦ {y | y.1 ∈ K i j}, fun i j ↦ ?_, ?_⟩
+      · simp only [memProd, q'']
         rcases Set.eq_empty_or_nonempty (K i j) with hK_empty | hK_nonempty
         · simp only [hK_empty, Set.mem_empty_iff_false, Set.setOf_false]
           exact ⟨∅, by simp [hq_empty]⟩
@@ -244,13 +244,13 @@ lemma IsPavingAnalyticFor.inter {𝓚' : Type*} {t : Set 𝓧}
         simp only [hB_eq, Set.mem_iInter, Set.mem_iUnion, Set.mem_prod, Set.mem_setOf_eq, C]
     · rw [← memProdSigmaDelta]
       simp_rw [memProdSigmaDelta_iff] at hB'_prod ⊢
-      choose A K hA hK hB_eq using hB'_prod
-      refine ⟨A, fun i j ↦ {y | y.2 ∈ K i j}, hA, fun i j ↦ ?_, ?_⟩
-      · simp only [memProd, exists_and_left, q'']
+      choose A hA K hK hB_eq using hB'_prod
+      refine ⟨A, hA, fun i j ↦ {y | y.2 ∈ K i j}, fun i j ↦ ?_, ?_⟩
+      · simp only [memProd, q'']
         rcases Set.eq_empty_or_nonempty (K i j) with hK_empty | hK_nonempty
         · simp only [hK_empty, Set.mem_empty_iff_false, Set.setOf_false]
           exact ⟨∅, by simp [hq_empty]⟩
-        simp only [Set.mem_insert_iff, exists_eq_or_imp, Set.univ_prod_univ, Set.mem_setOf_eq]
+        simp only [Set.mem_image2, Set.mem_insert_iff, exists_eq_or_imp, Set.univ_prod_univ]
         left
         right
         refine ⟨K i j, ?_⟩
@@ -300,8 +300,8 @@ lemma IsPavingAnalyticFor.union {𝓚' : Type*} {t : Set 𝓧}
     rw [hC_eq]
     refine memDelta.iInter fun k ↦ memDelta_of_mem ?_
     simp_rw [memSigma_memProd_iff] at hA hA'
-    choose B K hB hK hA_eq using hA
-    choose B' K' hB' hK' hA'_eq using hA'
+    choose B hB K hK hA_eq using hA
+    choose B' hB' K' hK' hA'_eq using hA'
     simp_rw [hA_eq, hA'_eq]
     have h_eq : (Equiv.prodSumDistrib 𝓧 𝓚 𝓚').symm '' Set.sumEquiv.symm
           (⋃ n, B k n ×ˢ K k n, ⋃ n, B' k n ×ˢ K' k n)
@@ -321,7 +321,7 @@ lemma IsPavingAnalyticFor.union {𝓚' : Type*} {t : Set 𝓧}
       Equiv.coe_fn_symm_mk]
     rw [Set.image_union]
     refine memSigma.union (memSigma_of_mem ?_) (memSigma_of_mem ?_)
-    · refine ⟨B k i, Sum.inl '' (K k i), hB _ _, ?_, ?_⟩
+    · refine ⟨B k i, hB _ _, Sum.inl '' (K k i), ?_, ?_⟩
       · simp only [Set.mem_insert_iff, Set.preimage_eq_univ_iff, Set.mem_setOf_eq,
           Set.preimage_inr_image_inl, q'']
         refine ⟨.inr ?_, .inr hq'_empty⟩
@@ -331,7 +331,7 @@ lemma IsPavingAnalyticFor.union {𝓚' : Type*} {t : Set 𝓧}
       · ext
         simp [Equiv.prodSumDistrib]
         grind
-    · refine ⟨B' k i, Sum.inr '' (K' k i), hB' _ _, ?_, ?_⟩
+    · refine ⟨B' k i, hB' _ _, Sum.inr '' (K' k i), ?_, ?_⟩
       · simp only [Set.mem_insert_iff, Set.preimage_eq_univ_iff, Set.mem_setOf_eq,
           Set.preimage_inl_image_inr, q'']
         refine ⟨.inr hq_empty, .inr ?_⟩
@@ -383,12 +383,12 @@ lemma IsPavingAnalyticFor.fst {𝓚' : Type*} (hq_empty : ∅ ∈ q) (hq : IsCom
     IsPavingAnalyticFor p (𝓚 × 𝓚') (Prod.fst '' s) := by
   obtain ⟨q', hq'_empty, hq', K, hK, rfl⟩ := hs
   refine ⟨memProd q q', ?_, hq.memProd hq', Equiv.prodAssoc 𝓧 𝓚 𝓚' '' K, ?_, by ext; simp⟩
-  · exact ⟨∅, ∅, hq_empty, hq'_empty, by simp⟩
+  · exact ⟨∅, hq_empty, ∅, hq'_empty, by simp⟩
   simp_rw [memProdSigmaDelta_iff] at hK ⊢
-  obtain ⟨B, K', hB, hK', rfl⟩ := hK
-  choose A K hA hK h_eq using hB
-  refine ⟨A, fun n m ↦ K n m ×ˢ K' n m, hA, fun n m ↦ ?_, ?_⟩
-  · exact ⟨K n m, K' n m, hK n m, hK' n m, rfl⟩
+  obtain ⟨B, hB, K', hK', rfl⟩ := hK
+  choose A hA K hK h_eq using hB
+  refine ⟨A, hA, fun n m ↦ K n m ×ˢ K' n m, fun n m ↦ ?_, ?_⟩
+  · exact ⟨K n m, hK n m, K' n m, hK' n m, rfl⟩
   · rw [Set.image_iInter (Equiv.prodAssoc 𝓧 𝓚 𝓚').bijective]
     simp_rw [Set.image_iUnion]
     congr
@@ -415,9 +415,9 @@ lemma IsPavingAnalyticFor.prod_left {𝓨 : Type*} {r : Set 𝓨 → Prop} {t : 
     grind
   refine ⟨q, hq_empty, hq_compact, (Equiv.prodAssoc _ _ _).symm '' (t ×ˢ s'), ?_, h_eq'⟩
   simp_rw [memProdSigmaDelta_iff] at hs_prod ⊢
-  obtain ⟨A, K, hA, hK, rfl⟩ := hs_prod
-  refine ⟨fun n m ↦ t ×ˢ A n m, K, fun n m ↦ ?_, hK, ?_⟩
-  · exact ⟨t, A n m, ht, hA n m, rfl⟩
+  obtain ⟨A, hA, K, hK, rfl⟩ := hs_prod
+  refine ⟨fun n m ↦ t ×ˢ A n m, fun n m ↦ ?_, K, hK, ?_⟩
+  · exact ⟨t, ht, A n m, hA n m, rfl⟩
   · rw [Set.prod_iInter, Set.image_iInter (Equiv.prodAssoc _ _ _).symm.bijective]
     simp_rw [Set.prod_iUnion, Set.image_iUnion]
     congr
@@ -451,9 +451,9 @@ lemma IsPavingAnalyticFor.prod_right {𝓨 : Type*} {r : Set 𝓨 → Prop} {t :
   refine ⟨q, hq_empty, hq_compact, (Equiv.prodAssoc _ _ _).symm ''
       (Prod.map id Prod.swap '' ((Equiv.prodAssoc _ _ _) '' (s' ×ˢ t))), ?_, h_eq'⟩
   simp_rw [memProdSigmaDelta_iff] at hs_prod ⊢
-  obtain ⟨A, K, hA, hK, rfl⟩ := hs_prod
-  refine ⟨fun n m ↦ A n m ×ˢ t, K, fun n m ↦ ?_, hK, ?_⟩
-  · exact ⟨A n m, t, hA n m, ht, rfl⟩
+  obtain ⟨A, hA, K, hK, rfl⟩ := hs_prod
+  refine ⟨fun n m ↦ A n m ×ˢ t, fun n m ↦ ?_, K, hK, ?_⟩
+  · exact ⟨A n m, hA n m, t, ht, rfl⟩
   · rw [Set.iInter_prod, Set.image_iInter (Equiv.prodAssoc _ _ _).bijective,
       Set.image_iInter, Set.image_iInter (Equiv.prodAssoc _ _ _).symm.bijective]
     swap
@@ -471,25 +471,25 @@ lemma IsPavingAnalytic.prod_right {𝓨 : Type*} {r : Set 𝓨 → Prop} {t : Se
 lemma isPavingAnalyticFor_of_memProd_isPavingAnalyticFor_left {𝓨 : Type*} {r : Set 𝓨 → Prop}
     {t : Set (𝓨 × 𝓧)} (ht : t ∈ memProd r (IsPavingAnalyticFor p 𝓚)) :
     IsPavingAnalyticFor (memProd r p) 𝓚 t := by
-  obtain ⟨A, s, hA, hs, rfl⟩ := ht
+  obtain ⟨A, hA, s, hs, rfl⟩ := ht
   exact hs.prod_left hA
 
 lemma isPavingAnalytic_of_memProd_isPavingAnalytic_left {𝓨 : Type*} {r : Set 𝓨 → Prop}
     {t : Set (𝓨 × 𝓧)} (ht : t ∈ memProd r (IsPavingAnalytic p)) :
     IsPavingAnalytic (memProd r p) t := by
-  obtain ⟨A, s, hA, hs, rfl⟩ := ht
+  obtain ⟨A, hA, s, hs, rfl⟩ := ht
   exact hs.prod_left hA
 
 lemma isPavingAnalyticFor_of_memProd_isPavingAnalyticFor_right {𝓨 : Type*} {r : Set 𝓨 → Prop}
     {t : Set (𝓧 × 𝓨)} (ht : t ∈ memProd (IsPavingAnalyticFor p 𝓚) r) :
     IsPavingAnalyticFor (memProd p r) 𝓚 t := by
-  obtain ⟨A, s, hA, hs, rfl⟩ := ht
+  obtain ⟨A, hA, s, hs, rfl⟩ := ht
   exact hA.prod_right hs
 
 lemma isPavingAnalytic_of_memProd_isPavingAnalytic_right {𝓨 : Type*} {r : Set 𝓨 → Prop}
     {t : Set (𝓧 × 𝓨)} (ht : t ∈ memProd (IsPavingAnalytic p) r) :
     IsPavingAnalytic (memProd p r) t := by
-  obtain ⟨A, s, hA, hs, rfl⟩ := ht
+  obtain ⟨A, hA, s, hs, rfl⟩ := ht
   exact hA.prod_right hs
 
 lemma isPavingAnalyticFor_of_memSigma_memProd_isPavingAnalyticFor_left
@@ -575,8 +575,8 @@ lemma IsPavingAnalyticFor.inter_set (hs : IsPavingAnalyticFor p 𝓚 s) (t : Set
   let A' := (t ×ˢ .univ) ∩ A
   refine ⟨q, hq_empty, hq, A', ?_, ?_⟩
   · simp_rw [memProdSigmaDelta_iff] at hA ⊢
-    obtain ⟨B, K, hB, hK, rfl⟩ := hA
-    refine ⟨fun n m ↦ B n m ∩ t, K, fun n m ↦ ?_, hK, ?_⟩
+    obtain ⟨B, hB, K, hK, rfl⟩ := hA
+    refine ⟨fun n m ↦ B n m ∩ t, fun n m ↦ ?_, K, hK, ?_⟩
     · exact ⟨B n m, hB n m, rfl⟩
     · simp only [A']
       simp_rw [Set.inter_iInter, Set.inter_iUnion]
@@ -594,13 +594,13 @@ lemma exists_isPavingAnalyticFor_of_inter_set (t : Set 𝓧)
     ∃ s', IsPavingAnalyticFor p 𝓚 s' ∧ s = s' ∩ t := by
   obtain ⟨q, hq_empty, hq, A, hA, rfl⟩ := hs
   rw [memProdSigmaDelta_iff] at hA
-  obtain ⟨B, K, hB, hK, rfl⟩ := hA
+  obtain ⟨B, hB, K, hK, rfl⟩ := hA
   choose A' hA' hBA' using hB
   refine ⟨Prod.fst '' (⋂ n, ⋃ m, A' n m ×ˢ K n m), ?_, ?_⟩
   · refine ⟨q, hq_empty, hq, ?_⟩
     refine ⟨⋂ n, ⋃ m, A' n m ×ˢ K n m, ?_, rfl⟩
     rw [memProdSigmaDelta_iff]
-    exact ⟨A', K, hA', hK, rfl⟩
+    exact ⟨A', hA', K, hK, rfl⟩
   · simp only [hBA']
     have h_eq n m : (A' n m ∩ t) ×ˢ K n m = (A' n m ×ˢ K n m) ∩ (t ×ˢ .univ) := by
       ext; simp; grind
@@ -697,18 +697,18 @@ lemma aux_Icc (l u : ℝ) : (Set.Icc l u)ᶜ ∈ memSigma {t | ∃ a b, Set.Icc 
 lemma aux'_Icc [MeasurableSpace 𝓧] (s : Set (𝓧 × ℝ))
     (hs : s ∈ memProd MeasurableSet {t | ∃ a b, Set.Icc a b = t}) :
      sᶜ ∈ memSigma (memProd MeasurableSet {t | ∃ a b, Set.Icc a b = t}) := by
-  obtain ⟨A, K, hA, ⟨l, u, rfl⟩, rfl⟩ := hs
+  obtain ⟨A, hA, K, ⟨l, u, rfl⟩, rfl⟩ := hs
   have hK' := aux_Icc l u
   rw [Set.compl_prod_eq_union]
   refine memSigma.union ?_ ?_
   · obtain ⟨B, hB, h_eq⟩ := univ_memSigma_Icc
     rw [h_eq, Set.prod_iUnion]
     refine ⟨fun i ↦ Aᶜ ×ˢ B i, fun n ↦ ?_, rfl⟩
-    exact ⟨Aᶜ, B n, hA.compl, hB n, rfl⟩
+    exact ⟨Aᶜ, hA.compl, B n, hB n, rfl⟩
   · obtain ⟨B, hB, h_eq⟩ := aux_Icc l u
     rw [h_eq, Set.prod_iUnion]
     refine ⟨fun i ↦ Set.univ ×ˢ B i, fun n ↦ ?_, rfl⟩
-    exact ⟨Set.univ, B n, .univ, hB n, rfl⟩
+    exact ⟨Set.univ, .univ, B n, hB n, rfl⟩
 
 lemma borel_eq_generateFrom_isCompact : borel ℝ = MeasurableSpace.generateFrom IsCompact := by
   refine le_antisymm ?_ ?_
@@ -786,17 +786,14 @@ lemma _root_.MeasurableSet.isPavingAnalytic_memProd {s : Set (𝓧 × ℝ)} {m�
     swap
     · rw [Real.measurableSpace, borel_eq_generateFrom_Icc']
     rw [← h_prod_eq]
-    congr with s
-    simp only [memProd, eq_comm, Set.mem_setOf_eq, exists_and_left, ↓existsAndEq, true_and,
-      Set.mem_image2]
-    congr!
+    rfl
 
 -- Icc version of He 1.32 (2)
 lemma isPavingAnalytic_memProd_measurableSet_Icc_iff {s : Set (𝓧 × ℝ)} [MeasurableSpace 𝓧] :
     IsPavingAnalytic (memProd MeasurableSet {t | ∃ a b : ℝ, Set.Icc a b = t}) s ↔
       IsPavingAnalytic MeasurableSet s := by
   refine ⟨fun hs ↦ hs.mono fun s hs ↦ ?_, fun hs ↦ ?_⟩
-  · obtain ⟨A, K, hA, ⟨a, b, rfl⟩, rfl⟩ := hs
+  · obtain ⟨A, hA, K, ⟨a, b, rfl⟩, rfl⟩ := hs
     exact hA.prod measurableSet_Icc
   · exact isPavingAnalytic_isPavingAnalytic
       (hs.mono fun _ ↦ MeasurableSet.isPavingAnalytic_memProd)
